misc: Refactor Substitution.lean to snake case

Hybrid/Language/Substitution.lean
@@ -12,93 +12,93 @@ class Term (symbs : Symbols α) (β: symbs.signature.S → Type v) where
 
 namespace FormL
 
-def nomOccurs {symbs : Symbols α} {s : symbs.signature.S} {sorts : List symbs.signature.S} (i : symbs.nominal s): FormL symbs sorts → Bool
+def nom_occurs {symbs : Symbols α} {s : symbs.signature.S} {sorts : List symbs.signature.S} (i : symbs.nominal s): FormL symbs sorts → Bool
   | @FormL.nom  _ _ s' j   =>
       if h : s = s' then
         i == (h ▸ j)
       else false
   | @FormL.at _ _ s' _ j φ =>
-      nomOccurs i φ ||
+      nom_occurs i φ ||
         if h : s = s' then
           i == (h ▸ j)
         else false
-  | (φ, ψ)   => nomOccurs i φ || nomOccurs i ψ
-  | ℋ⟨_⟩ φ    => nomOccurs i φ
-  | φ ⋁ ψ    => nomOccurs i φ || nomOccurs i ψ
-  | ∼ φ      => nomOccurs i φ
-  | ℋ∀ _ φ  => nomOccurs i φ
+  | (φ, ψ)   => nom_occurs i φ || nom_occurs i ψ
+  | ℋ⟨_⟩ φ    => nom_occurs i φ
+  | φ ⋁ ψ    => nom_occurs i φ || nom_occurs i ψ
+  | ∼ φ      => nom_occurs i φ
+  | ℋ∀ _ φ  => nom_occurs i φ
   | _        => false
 
-def varOccurs {symbs : Symbols α} {s : symbs.signature.S} {sorts : List symbs.signature.S} (x : symbs.svar s): FormL symbs sorts → Bool
+def var_occurs {symbs : Symbols α} {s : symbs.signature.S} {sorts : List symbs.signature.S} (x : symbs.svar s): FormL symbs sorts → Bool
   | @FormL.svar  _ _ s' j   =>
       if h : s = s' then
         x == (h ▸ j)
       else false
   | @FormL.bind _ _ s' _ y φ =>
-      varOccurs y φ ||
+      var_occurs y φ ||
         if h : s = s' then
           x == (h ▸ y)
         else false
-  | (φ, ψ)   => varOccurs x φ || varOccurs x ψ
-  | ℋ⟨_⟩ φ    => varOccurs x φ
-  | φ ⋁ ψ    => varOccurs x φ || varOccurs x ψ
-  | ∼ φ      => varOccurs x φ
-  | ℋ@ _ φ  => varOccurs x φ
+  | (φ, ψ)   => var_occurs x φ || var_occurs x ψ
+  | ℋ⟨_⟩ φ    => var_occurs x φ
+  | φ ⋁ ψ    => var_occurs x φ || var_occurs x ψ
+  | ∼ φ      => var_occurs x φ
+  | ℋ@ _ φ  => var_occurs x φ
   | _        => false
 
 
 -- x occurs in φ, and x is free in φ
 @[simp]
-def varOccursFree {symbs : Symbols α} {s : symbs.signature.S} {sorts : List symbs.signature.S} (x : symbs.svar s): FormL symbs sorts → Bool
+def occurs_free {symbs : Symbols α} {s : symbs.signature.S} {sorts : List symbs.signature.S} (x : symbs.svar s): FormL symbs sorts → Bool
   | @FormL.bind _ _ s' _ y φ =>
       if h : s = s' then
         if x = (h ▸ y) then
           false
-        else varOccursFree x φ
-      else varOccursFree x φ
-  | (φ, ψ)   => varOccursFree x φ || varOccursFree x ψ
-  | ℋ⟨_⟩ φ    => varOccursFree x φ
-  | φ ⋁ ψ    => varOccursFree x φ || varOccursFree x ψ
-  | ∼ φ      => varOccursFree x φ
-  | ℋ@ _ φ  => varOccursFree x φ
-  | φ        => varOccurs x φ
+        else occurs_free x φ
+      else occurs_free x φ
+  | (φ, ψ)   => occurs_free x φ || occurs_free x ψ
+  | ℋ⟨_⟩ φ    => occurs_free x φ
+  | φ ⋁ ψ    => occurs_free x φ || occurs_free x ψ
+  | ∼ φ      => occurs_free x φ
+  | ℋ@ _ φ  => occurs_free x φ
+  | φ        => var_occurs x φ
 
 abbrev Context.all_else_not_free {symbs : Symbols α} {s s' : symbs.signature.S} {sorts : List symbs.signature.S} {φ : Form symbs s} {ψ : FormL symbs sorts} (x : symbs.svar s') (C : φ.Context ψ) : Bool :=
-  C.all_else_bool (λ φ => !φ.varOccursFree x)
+  C.all_else_bool (λ φ => !φ.occurs_free x)
 
 
 -- x occurs in φ, and x is bound in φ
-def varOccursBound {symbs : Symbols α} {s : symbs.signature.S} {sorts : List symbs.signature.S} (x : symbs.svar s): FormL symbs sorts → Bool
+def occurs_bound {symbs : Symbols α} {s : symbs.signature.S} {sorts : List symbs.signature.S} (x : symbs.svar s): FormL symbs sorts → Bool
   | @FormL.bind _ _ s' _ y φ =>
       if h : s = s' then
         if x = (h ▸ y) then
           true
-        else varOccursBound x φ
-      else varOccursBound x φ
-  | (φ, ψ)   => varOccursBound x φ || varOccursBound x ψ
-  | ℋ⟨_⟩ φ    => varOccursBound x φ
-  | φ ⋁ ψ    => varOccursBound x φ || varOccursBound x ψ
-  | ∼ φ      => varOccursBound x φ
-  | ℋ@ _ φ   => varOccursBound x φ
+        else occurs_bound x φ
+      else occurs_bound x φ
+  | (φ, ψ)   => occurs_bound x φ || occurs_bound x ψ
+  | ℋ⟨_⟩ φ    => occurs_bound x φ
+  | φ ⋁ ψ    => occurs_bound x φ || occurs_bound x ψ
+  | ∼ φ      => occurs_bound x φ
+  | ℋ@ _ φ   => occurs_bound x φ
   | _        => false
 
 -- x is substitutable for y in φ
-def varSubstableFor {symbs : Symbols α} {s : symbs.signature.S} {sorts : List symbs.signature.S} (x y : symbs.svar s): FormL symbs sorts → Bool
+def free_for {symbs : Symbols α} {s : symbs.signature.S} {sorts : List symbs.signature.S} (x y : symbs.svar s): FormL symbs sorts → Bool
   | @FormL.bind _ _ s' _ z φ =>
-    if !φ.varOccursFree y then
+    if !φ.occurs_free y then
       true
-    else varSubstableFor x y φ &&
+    else free_for x y φ &&
       if h : s = s' then
         x != (h ▸ z)
       else true
-  | (φ, ψ)   => varSubstableFor x y φ && varSubstableFor x y ψ
-  | ℋ⟨_⟩ φ    => varSubstableFor x y φ
-  | φ ⋁ ψ   => varSubstableFor x y φ && varSubstableFor x y ψ
-  | ∼ φ      => varSubstableFor x y φ
-  | ℋ@ _ φ   => varSubstableFor x y φ
+  | (φ, ψ)   => free_for x y φ && free_for x y ψ
+  | ℋ⟨_⟩ φ    => free_for x y φ
+  | φ ⋁ ψ   => free_for x y φ && free_for x y ψ
+  | ∼ φ      => free_for x y φ
+  | ℋ@ _ φ   => free_for x y φ
   | _        => true
 
-def varSubst {symbs : Symbols α} {s : symbs.signature.S} {sorts : List symbs.signature.S} (x y : symbs.svar s): FormL symbs sorts → FormL symbs sorts
+def var_subst {symbs : Symbols α} {s : symbs.signature.S} {sorts : List symbs.signature.S} (x y : symbs.svar s): FormL symbs sorts → FormL symbs sorts
   | @FormL.svar _ _ s' z   =>
       if h : s = s' then
         if (y = h ▸ z) then
@@ -113,16 +113,16 @@ def varSubst {symbs : Symbols α} {s : symbs.signature.S} {sorts : List symbs.si
         --  If z = x and y is free in φ, this function will capture
         --  y in (∀ z. φ)[x / y]
         -- Safety is guaranteed only if a proof of (y is free for x in φ) is also given in the context.
-        else ℋ∀z (varSubst x y φ)
-      else ℋ∀z (varSubst x y φ)
-  | (φ, ψ)   => (varSubst x y φ, varSubst x y ψ)
-  | ℋ⟨σ⟩ φ    => ℋ⟨σ⟩ (varSubst x y φ)
-  | φ ⋁ ψ    => (varSubst x y φ) ⋁ (varSubst x y ψ)
-  | ∼ φ      => ∼ (varSubst x y φ)
-  | ℋ@k φ   => ℋ@k (varSubst x y φ)
+        else ℋ∀z (var_subst x y φ)
+      else ℋ∀z (var_subst x y φ)
+  | (φ, ψ)   => (var_subst x y φ, var_subst x y ψ)
+  | ℋ⟨σ⟩ φ    => ℋ⟨σ⟩ (var_subst x y φ)
+  | φ ⋁ ψ    => (var_subst x y φ) ⋁ (var_subst x y ψ)
+  | ∼ φ      => ∼ (var_subst x y φ)
+  | ℋ@k φ   => ℋ@k (var_subst x y φ)
   | φ => φ
 
-def nomSubst {symbs : Symbols α} {s : symbs.signature.S} {sorts : List symbs.signature.S} (i : symbs.nominal s) (y : symbs.svar s): FormL symbs sorts → FormL symbs sorts
+def nom_subst {symbs : Symbols α} {s : symbs.signature.S} {sorts : List symbs.signature.S} (i : symbs.nominal s) (y : symbs.svar s): FormL symbs sorts → FormL symbs sorts
   | @FormL.svar _ _ s' z   =>
       if h : s = s' then
         if (y = h ▸ z) then
@@ -133,23 +133,23 @@ def nomSubst {symbs : Symbols α} {s : symbs.signature.S} {sorts : List symbs.si
       if h : s = s' then
         if (y = h ▸ z) then
           ℋ∀z φ
-        else ℋ∀z (nomSubst i y φ)
-      else ℋ∀z (nomSubst i y φ)
-  | (φ, ψ)   => (nomSubst i y φ, nomSubst i y ψ)
-  | ℋ⟨σ⟩ φ    => ℋ⟨σ⟩ (nomSubst i y φ)
-  | φ ⋁ ψ    => (nomSubst i y φ) ⋁ (nomSubst i y ψ)
-  | ∼ φ      => ∼ (nomSubst i y φ)
-  | ℋ@k φ   => ℋ@k (nomSubst i y φ)
+        else ℋ∀z (nom_subst i y φ)
+      else ℋ∀z (nom_subst i y φ)
+  | (φ, ψ)   => (nom_subst i y φ, nom_subst i y ψ)
+  | ℋ⟨σ⟩ φ    => ℋ⟨σ⟩ (nom_subst i y φ)
+  | φ ⋁ ψ    => (nom_subst i y φ) ⋁ (nom_subst i y ψ)
+  | ∼ φ      => ∼ (nom_subst i y φ)
+  | ℋ@k φ   => ℋ@k (nom_subst i y φ)
   | φ => φ
 
 
 instance {symbs : Symbols α} : Term symbs symbs.nominal where
-  occurs := FormL.nomOccurs
-  subst  := FormL.nomSubst
+  occurs := nom_occurs
+  subst  := nom_subst
 
 instance {symbs : Symbols α} : @Term α symbs symbs.svarType where
-  occurs := FormL.varOccurs
-  subst  := FormL.varSubst
+  occurs := var_occurs
+  subst  := var_subst
 
 notation:max φ:lead "[" x:arg "//" y:arg "]" => Term.subst x y φ
 
@@ -167,94 +167,94 @@ variable {σ : symbs.signature.Sig (t :: sorts) u}
 
 @[simp]
 lemma subst_var_appl : (ℋ⟨σ⟩ φ)[y // x] = ℋ⟨σ⟩ (φ[y // x]) := by
-  simp only [Term.subst, varSubst]
+  simp only [Term.subst, var_subst]
 
 @[simp]
 lemma subst_nom_appl : (ℋ⟨σ⟩ φ)[i // x] = ℋ⟨σ⟩ (φ[i // x]) := by
-  simp only [Term.subst, nomSubst]
+  simp only [Term.subst, nom_subst]
 
 @[simp]
 lemma subst_var_or : (φ ⋁ ψ)[y // x] = φ[y // x] ⋁ ψ[y // x] := by
-  simp only [Term.subst, varSubst]
+  simp only [Term.subst, var_subst]
 
 @[simp]
 lemma subst_nom_or : (φ ⋁ ψ)[i // x] = φ[i // x] ⋁ ψ[i // x] := by
-  simp only [Term.subst, nomSubst]
+  simp only [Term.subst, nom_subst]
 
 @[simp]
 lemma subst_var_neg : (∼φ)[y // x] = ∼(φ[y // x]) := by
-  simp only [Term.subst, varSubst]
+  simp only [Term.subst, var_subst]
 
 @[simp]
 lemma subst_nom_neg : (∼φ)[i // x] = ∼(φ[i // x]) := by
-  simp only [Term.subst, nomSubst]
+  simp only [Term.subst, nom_subst]
 
 @[simp]
 lemma subst_var_at {φ : Form symbs t} {k : symbs.nominal t} : (@FormL.at α symbs t u k φ)[y // x] = (ℋ@ k (φ[y // x])) := by
-  simp only [Term.subst, varSubst]
+  simp only [Term.subst, var_subst]
 
 @[simp]
 lemma subst_nom_at {φ : Form symbs t} {k : symbs.nominal t} : (@FormL.at α symbs t u k φ)[j // x] = (ℋ@ k (φ[j // x])) := by
-  simp only [Term.subst, nomSubst]
+  simp only [Term.subst, nom_subst]
 
 @[simp]
 lemma subst_var_cons {φ : Form symbs t} : (φ, ψ)[y // x] = (φ[y // x], ψ[y // x]) := by
-  simp only [Term.subst, varSubst]
+  simp only [Term.subst, var_subst]
 
 @[simp]
 lemma subst_nom_cons {φ : Form symbs t} : (φ, ψ)[i // x] = (φ[i // x], ψ[i // x]) := by
-  simp only [Term.subst, nomSubst]
+  simp only [Term.subst, nom_subst]
 
 @[simp]
 lemma subst_var_bind_neq_sorts {z : symbs.svar t} (h : ¬s = t) : (ℋ∀ z φ)[y // x] = ℋ∀ z (φ[y // x]) := by
-  simp only [Term.subst, varSubst, h, ↓reduceDIte]
+  simp only [Term.subst, var_subst, h, ↓reduceDIte]
 
 @[simp]
 lemma subst_var_bind_neq_vars {z : symbs.svar s} (h : ¬x = z) : (ℋ∀ z φ)[y // x] = ℋ∀ z (φ[y // x]) := by
-  simp only [Term.subst, varSubst, ↓reduceDIte, h, ↓reduceIte]
+  simp only [Term.subst, var_subst, ↓reduceDIte, h, ↓reduceIte]
 
 @[simp]
 lemma subst_var_bind : (ℋ∀ x φ)[y // x] = ℋ∀ x φ := by
-  simp only [Term.subst, varSubst, ↓reduceDIte, ↓reduceIte]
+  simp only [Term.subst, var_subst, ↓reduceDIte, ↓reduceIte]
 
 end CongrLemmas
 
-lemma notFreeBound {symbs : Symbols α} {s t u : symbs.signature.S} {x : symbs.svarType s} {y : symbs.svarType t} {φ : Form symbs u} (h : φ.varOccursFree x = false): (ℋ∀ y φ).varOccursFree x = false := by
-  simp only [varOccursFree, h, ite_self, dite_eq_ite]
+lemma not_free_bound {symbs : Symbols α} {s t u : symbs.signature.S} {x : symbs.svarType s} {y : symbs.svarType t} {φ : Form symbs u} (h : φ.occurs_free x = false): (ℋ∀ y φ).occurs_free x = false := by
+  simp only [occurs_free, h, ite_self, dite_eq_ite]
 
-lemma notFreeBound' {symbs : Symbols α} {s t : symbs.signature.S} {x : symbs.svarType s} {φ : Form symbs t}: (ℋ∀ x φ).varOccursFree x = false := by
-  simp only [varOccursFree, ↓reduceDIte, ↓reduceIte]
+lemma not_free_bound' {symbs : Symbols α} {s t : symbs.signature.S} {x : symbs.svarType s} {φ : Form symbs t}: (ℋ∀ x φ).occurs_free x = false := by
+  simp only [occurs_free, ↓reduceDIte, ↓reduceIte]
 
-lemma notFreeVarSubst {symbs : Symbols α} {s : symbs.signature.S} {sorts : List symbs.signature.S} {x y : symbs.svarType s} {φ : FormL symbs sorts} (h : φ.varOccursFree x = false): φ[y // x] = φ := by
+lemma not_free_var_subst {symbs : Symbols α} {s : symbs.signature.S} {sorts : List symbs.signature.S} {x y : symbs.svarType s} {φ : FormL symbs sorts} (h : φ.occurs_free x = false): φ[y // x] = φ := by
   induction φ with
   | bind z φ ih =>
       rename_i t _
       by_cases eq_sorts : s = t
       . subst eq_sorts
-        simp [Term.subst, varSubst] at ih ⊢
-        simp [varOccursFree] at h
+        simp [Term.subst, var_subst] at ih ⊢
+        simp [occurs_free] at h
         intro h2
         apply ih
         apply h
         exact h2
       . simp only [eq_sorts, not_false_eq_true, subst_var_bind_neq_sorts, bind.injEq, heq_eq_eq,
         true_and]
-        simp only [varOccursFree, eq_sorts, ↓reduceDIte] at h
+        simp only [occurs_free, eq_sorts, ↓reduceDIte] at h
         exact ih h
   | svar z =>
-      simp [varOccursFree, varOccurs] at h
-      simp [Term.subst, varSubst]
+      simp [occurs_free, var_occurs] at h
+      simp [Term.subst, var_subst]
       intro h2
       specialize h h2
       intro v
       subst v
       contradiction
   | appl σ ψ ih =>
-      simp [Term.subst, varSubst]
+      simp [Term.subst, var_subst]
       apply ih
       exact h
   | or φ ψ ih1 ih2 =>
-      simp [Term.subst, varSubst]
+      simp [Term.subst, var_subst]
       simp at h
       apply And.intro
       . apply ih1
@@ -262,11 +262,11 @@ lemma notFreeVarSubst {symbs : Symbols α} {s : symbs.signature.S} {sorts : List
       . apply ih2
         exact h.2
   | neg φ ih =>
-      simp [Term.subst, varSubst]
+      simp [Term.subst, var_subst]
       apply ih
       exact h
   | cons φ ψs ih1 ih2 =>
-      simp [Term.subst, varSubst]
+      simp [Term.subst, var_subst]
       simp at h
       apply And.intro
       . apply ih1
@@ -274,13 +274,13 @@ lemma notFreeVarSubst {symbs : Symbols α} {s : symbs.signature.S} {sorts : List
       . apply ih2
         exact h.2
   | «at» k _ ih =>
-      simp [Term.subst, varSubst]
+      simp [Term.subst, var_subst]
       apply ih
       exact h
-  | _ => simp [Term.subst, varSubst] at h ⊢
+  | _ => simp [Term.subst, var_subst] at h ⊢
 
-lemma notFreeVarSubst' {symbs : Symbols α} {s : symbs.signature.S} {sorts : List symbs.signature.S} {x y : symbs.svarType s} {φ : FormL symbs sorts} (h : φ.varOccursFree x = false): φ.varSubst y x = φ := by
-  apply notFreeVarSubst
+lemma not_free_var_subst' {symbs : Symbols α} {s : symbs.signature.S} {sorts : List symbs.signature.S} {x y : symbs.svarType s} {φ : FormL symbs sorts} (h : φ.occurs_free x = false): φ.var_subst y x = φ := by
+  apply not_free_var_subst
   exact h
 
 end FormL
